src/Encoding/ModularWordEncodingTheorems.v
@@ -3,7 +3,7 @@ Require Import Coq.Numbers.Natural.Peano.NPeano.
 Require Import Crypto.CompleteEdwardsCurve.CompleteEdwardsCurveTheorems.
 Require Import Crypto.ModularArithmetic.PrimeFieldTheorems Crypto.ModularArithmetic.ModularArithmeticTheorems.
 Require Import Bedrock.Word.
-Require Import Crypto.Tactics.VerdiTactics.
+Require Import Crypto.Tactics.VerdiTactics Crypto.Util.Tactics.
 Require Import Crypto.Spec.Encoding.
 Require Import Crypto.Util.ZUtil.
 Require Import Crypto.Spec.ModularWordEncoding.
@@ -24,7 +24,7 @@ Section SignBit.
       assert (m < 1)%Z by (apply Z2Nat.inj_lt; try omega; assumption).
       omega.
     + assert (0 < m)%Z as m_pos by (pose proof prime_ge_2 m prime_m; omega).
-      pose proof (FieldToZ_range x m_pos).
+      pose proof (Zmod.FieldToZ_range x m_pos).
       destruct (FieldToZ x); auto.
       - destruct p; auto.
       - pose proof (Pos2Z.neg_is_neg p); omega.
@@ -35,20 +35,13 @@ Section SignBit.
     rewrite sign_bit_parity; auto.
   Qed.
 
-  Lemma sign_bit_opp : forall (x : F m), x <> 0 -> negb (@sign_bit m sz x) = @sign_bit m sz (opp x).
-  Proof.
-    intros.
-    pose proof sign_bit_zero as sign_zero.
-    rewrite !sign_bit_parity in *.
-    pose proof (F_opp_spec x) as opp_spec_x.
-    apply F_eq in opp_spec_x.
-    rewrite FieldToZ_add in opp_spec_x.
-    rewrite <-opp_spec_x, Z.odd_mod in sign_zero by (pose proof prime_ge_2 m prime_m; omega).
-    replace (Z.odd m) with true in sign_zero by (destruct (Z.prime_odd_or_2 m prime_m); auto || omega).
-    rewrite Z.odd_add, F_FieldToZ_add_opp, Z.div_same, Bool.xorb_true_r in sign_zero by assumption || omega.
-    apply Bool.xorb_eq.
-    rewrite <-Bool.negb_xorb_l.
-    assumption.
-  Qed.
+  Lemma odd_m : Z.odd m = true. Admitted.
 
+  Lemma sign_bit_opp (x : F m) (Hnz:x <> 0) : negb (@sign_bit m sz x) = @sign_bit m sz (opp x).
+  Proof.
+    pose proof Zmod.FieldToZ_nonzero_range x Hnz; specialize_by omega.
+    rewrite !sign_bit_parity, Zmod.FieldToZ_opp, Z_mod_nz_opp_full,
+      Zmod_small, Z.odd_sub, odd_m, (Bool.xorb_true_l (Z.odd x)) by
+       (omega || rewrite Zmod_small by omega; auto using Zmod.FieldToZ_nonzero); trivial.
+  Qed.
 End SignBit.
