src/ModularArithmetic/Tutorial.v
@@ -11,17 +11,16 @@ Section Mod24.
   Let q := 24.
 
   (* Boilerplate for letting Z numbers be interpreted as field elements *)
-  Let ZToFq := ZToField : BinNums.Z -> F q. Hint Unfold ZToFq. Local Coercion ZToFq : Z >-> F.
+  Let ZToFq := ZToField _ : BinNums.Z -> F q. Hint Unfold ZToFq. Local Coercion ZToFq : Z >-> F.
 
   (* Boilerplate for [ring]. Similar boilerplate works for [field] if
   the modulus is prime . *)
-  Add Ring Fring_q : (@Fring_theory q)
-    (morphism (@Fring_morph q),
-     preprocess [unfold ZToFq; Fpreprocess],
-     postprocess [Fpostprocess; try exact Fq_1_neq_0; try assumption],
-     constants [Fconstant],
-     div (@Fmorph_div_theory q),
-     power_tac (@Fpower_theory q) [Fexp_tac]).
+  Add Ring _theory : (Zmod.ring_theory q)
+    (morphism (Zmod.ring_morph q),
+     preprocess [unfold ZToFq],
+     constants [Zmod.is_constant],
+     div (Zmod.morph_div_theory q),
+     power_tac (Zmod.power_theory q) [Zmod.is_pow_constant]).
 
   Lemma sumOfSquares : forall a b: F q, (a+b)^2 = a^2 + 2*a*b + b^2.
   Proof.
@@ -39,34 +38,33 @@ Section Modq.
   Local Open Scope F_scope.
 
   (* Boilerplate for letting Z numbers be interpreted as field elements *)
-  Let ZToFq := ZToField : BinNums.Z -> F q. Hint Unfold ZToFq. Local Coercion ZToFq : Z >-> F.
+  Let ZToFq := ZToField _ : BinNums.Z -> F q. Hint Unfold ZToFq. Local Coercion ZToFq : Z >-> F.
 
   (* Boilerplate for [field]. Similar boilerplate works for [ring] if
   the modulus is not prime . *)
-  Add Field Ffield_q' : (@Ffield_theory q _)
-    (morphism (@Fring_morph q),
-     preprocess [unfold ZToFq; Fpreprocess],
-     postprocess [Fpostprocess; try exact Fq_1_neq_0; try assumption],
-     constants [Fconstant],
-     div (@Fmorph_div_theory q),
-     power_tac (@Fpower_theory q) [Fexp_tac]).
+  Add Field _theory' : (Zmod.field_theory q)
+    (morphism (Zmod.ring_morph q),
+     preprocess [unfold ZToFq],
+     constants [Zmod.is_constant],
+     div (Zmod.morph_div_theory q),
+     power_tac (Zmod.power_theory q) [Zmod.is_pow_constant]).
 
-  Lemma sumOfSquares' : forall a b c: F q, c <> 0 -> ((a+b)/c)^2 = a^2/c^2 + ZToField 2*(a/c)*(b/c) + b^2/c^2.
+  Lemma sumOfSquares' : forall a b c: F q, c <> 0 -> ((a+b)/c)^2 = a^2/c^2 + 2*(a/c)*(b/c) + b^2/c^2.
   Proof.
     intros.
-    field.
+    field; trivial.
   Qed.
 End Modq.
 
 (*** The old way: Modules ***)
 
-Module Modulus31 <: PrimeModulus.
+Module Modulus31 <: Zmod.PrimeModulus.
   Definition modulus := 2^5 - 1.
   Lemma prime_modulus : prime modulus.
   Admitted.
 End Modulus31.
 
-Module Modulus127 <: PrimeModulus.
+Module Modulus127 <: Zmod.PrimeModulus.
   Definition modulus := 2^127 - 1.
   Lemma prime_modulus : prime modulus.
   Admitted.
@@ -74,14 +72,14 @@ End Modulus127.
 
 Module Example31.
   (* Then we can construct a field with that modulus *)
-  Module Import Field := FieldModulo Modulus31.
+  Module Import Field := Zmod.FieldModulo Modulus31.
   Import Modulus31.
 
   (* And pull in the appropriate notations *)
   Local Open Scope F_scope.
 
   (* First, let's solve a ring example*)
-  Lemma ring_example: forall x: F modulus, x * (ZToField 2) = x + x.
+  Lemma ring_example: forall x: F modulus, x * (ZToField _ 2) = x + x.
   Proof.
     intros.
     ring.
@@ -92,7 +90,7 @@ Module Example31.
     Therefore, it is necessary to explicitly rewrite the modulus
     (usually hidden by implicitn arguments) match the one passed to
     [FieldModulo]. *)
-  Lemma ring_example': forall x: F (2^5-1), x * (ZToField 2) = x + x.
+  Lemma ring_example': forall x: F (2^5-1), x * (ZToField _ 2) = x + x.
   Proof.
     intros.
     change (2^5-1)%Z with modulus.
@@ -108,7 +106,7 @@ Module Example31.
   Qed.
 
   (* Then an example with exponentiation *)
-  Lemma exp_example: forall x: F modulus, x ^ 2 + ZToField 2 * x + 1 = (x + 1) ^ 2.
+  Lemma exp_example: forall x: F modulus, x ^ 2 + ZToField _ 2 * x + 1 = (x + 1) ^ 2.
   Proof.
     intros; simpl.
     field; trivial.
@@ -143,7 +141,7 @@ End Example31.
 
 (* Notice that the field tactics work whether we know what the modulus is *)
 Module TimesZeroTransparentTestModule.
-  Module Import Theory := FieldModulo Modulus127.
+  Module Import Theory := Zmod.FieldModulo Modulus127.
   Import Modulus127.
   Local Open Scope F_scope.
 
@@ -153,9 +151,13 @@ Module TimesZeroTransparentTestModule.
   Qed.
 End TimesZeroTransparentTestModule.
 
-(* Or if we don't (i.e. it's opaque) *)
-Module TimesZeroParametricTestModule (M: PrimeModulus).
-  Module Theory := FieldModulo M.
+(* An opaque modulus causes the field tactic to expand all constants
+  into matches on the modulus. Goals can still be proven, but with
+  significant overhead. Consider using an entirely abstract
+  [Algebra.field] instead. *)
+  
+Module TimesZeroParametricTestModule (M: Zmod.PrimeModulus).
+  Module Theory := Zmod.FieldModulo M.
   Import Theory M.
   Local Open Scope F_scope.
 
@@ -164,26 +166,27 @@ Module TimesZeroParametricTestModule (M: PrimeModulus).
     field.
   Qed.
 
-  Lemma realisticFraction : forall x y d : F modulus, (x * 1 + y * 0) / (1 + d * x * 0 * y * 1) = x.
-  Proof.
-    intros.
-    field; try exact Fq_1_neq_0.
-  Qed.
-
-  Lemma biggerFraction : forall XP YP ZP TP XQ YQ ZQ TQ d : F modulus,
-   ZQ <> 0 ->
-   ZP <> 0 ->
-   ZP * ZQ * ZP * ZQ + d * XP * XQ * YP * YQ <> 0 ->
-   ZP * ZToField 2 * ZQ * (ZP * ZQ) + XP * YP * ZToField 2 * d * (XQ * YQ) <> 0 ->
-   ZP * ZToField 2 * ZQ * (ZP * ZQ) - XP * YP * ZToField 2 * d * (XQ * YQ) <> 0 ->
-
-   ((YP + XP) * (YQ + XQ) - (YP - XP) * (YQ - XQ)) *
-   (ZP * ZToField 2 * ZQ - XP * YP / ZP * ZToField 2 * d * (XQ * YQ / ZQ)) /
-   ((ZP * ZToField 2 * ZQ - XP * YP / ZP * ZToField 2 * d * (XQ * YQ / ZQ)) *
-    (ZP * ZToField 2 * ZQ + XP * YP / ZP * ZToField 2 * d * (XQ * YQ / ZQ))) =
-   (XP / ZP * (YQ / ZQ) + YP / ZP * (XQ / ZQ)) / (1 + d * (XP / ZP) * (XQ / ZQ) * (YP / ZP) * (YQ / ZQ)).
+  Lemma realisticFraction : forall x y d : F modulus, 1 <> ZToField modulus 0 -> (x * 1 + y * 0) / (1 + d * x * 0 * y * 1) = x.
   Proof.
     intros.
     field; assumption.
+  Qed.
+
+  Lemma biggerFraction : forall XP YP ZP TP XQ YQ ZQ TQ d : F modulus,
+   1 <> ZToField modulus 0 -> 
+   ZQ <> 0 ->
+   ZP <> 0 ->
+   ZP * ZQ * ZP * ZQ + d * XP * XQ * YP * YQ <> 0 ->
+   ZP * ZToField _ 2 * ZQ * (ZP * ZQ) + XP * YP * ZToField _ 2 * d * (XQ * YQ) <> 0 ->
+   ZP * ZToField _ 2 * ZQ * (ZP * ZQ) - XP * YP * ZToField _ 2 * d * (XQ * YQ) <> 0 ->
+
+   ((YP + XP) * (YQ + XQ) - (YP - XP) * (YQ - XQ)) *
+   (ZP * ZToField _ 2 * ZQ - XP * YP / ZP * ZToField _ 2 * d * (XQ * YQ / ZQ)) /
+   ((ZP * ZToField _ 2 * ZQ - XP * YP / ZP * ZToField _ 2 * d * (XQ * YQ / ZQ)) *
+    (ZP * ZToField _ 2 * ZQ + XP * YP / ZP * ZToField _ 2 * d * (XQ * YQ / ZQ))) =
+   (XP / ZP * (YQ / ZQ) + YP / ZP * (XQ / ZQ)) / (1 + d * (XP / ZP) * (XQ / ZQ) * (YP / ZP) * (YQ / ZQ)).
+  Proof.
+    intros.
+    field; repeat split; assumption.
   Qed.
 End TimesZeroParametricTestModule.
